Update tutorial files

tutorial/ParallelIncrement.fst
@@ -1,63 +1,84 @@
+(*
+   Copyright 2023 Microsoft Research
+
+   Licensed under the Apache License, Version 2.0 (the "License");
+   you may not use this file except in compliance with the License.
+   You may obtain a copy of the License at
+
+       http://www.apache.org/licenses/LICENSE-2.0
+
+   Unless required by applicable law or agreed to in writing, software
+   distributed under the License is distributed on an "AS IS" BASIS,
+   WITHOUT WARRANTIES OR CONDITIONS OF ANY KIND, either express or implied.
+   See the License for the specific language governing permissions and
+   limitations under the License.
+*)
+
 module ParallelIncrement
+#lang-pulse
 open Pulse.Lib.Pervasives
-module U32 = FStar.UInt32
+
 module L = Pulse.Lib.SpinLock
 module GR = Pulse.Lib.GhostReference
 module R = Pulse.Lib.Reference
-```pulse
-fn increment (x: ref nat)
-             (l:L.lock (exists* v. pts_to x #one_half v))
-requires pts_to x #one_half 'i
-ensures pts_to x #one_half ('i + 1)
+
+
+fn increment (#p:perm)
+             (x:ref nat)
+             (l:L.lock)
+requires (L.lock_alive l #p (exists* v. pts_to x #0.5R v)) ** R.pts_to x #0.5R 'i
+ensures  (L.lock_alive l #p (exists* v. pts_to x #0.5R v)) ** R.pts_to x #0.5R ('i + 1)
  {
     let v = !x;
     L.acquire l;
     R.gather x;
-    with p _v. rewrite (pts_to x #p _v) as (pts_to x _v);
+    with p _v. rewrite (R.pts_to x #p _v) as (R.pts_to x _v);
     x := (v + 1);
     R.share x;
-    with p _v. rewrite (pts_to x #p _v) as (pts_to x #one_half _v);
+    with p _v. rewrite (R.pts_to x #p _v) as (R.pts_to x #0.5R _v);
     L.release l;
-    with p _v. rewrite (pts_to x #p _v) as (pts_to x #one_half _v);
+    with p _v. rewrite (R.pts_to x #p _v) as (R.pts_to x #0.5R _v);
 }
-```
 
-#push-options "--print_implicits --ext 'pulse:env_on_err' --print_full_names"
-```pulse
+
 fn increment_f (x: ref nat)
-               (#pred #qpred: nat -> vprop)
-               (l:L.lock (exists* v. pts_to x #one_half v ** pred v))
-               (f: (v:nat -> stt_ghost unit emp_inames 
-                        (pred v ** qpred v ** pts_to x #one_half (v + 1))
-                        (fun _ -> pred (v + 1) ** qpred (v + 1) ** pts_to x #one_half (v + 1))))
-requires pts_to x #one_half 'i ** qpred 'i
-ensures pts_to x #one_half ('i + 1) ** qpred ('i + 1)
+               (#p:perm)
+               (#pred #qpred: nat -> slprop)
+               (l:L.lock)
+               (f: (v:nat -> stt_ghost unit
+                        emp_inames
+                        (pred v ** qpred v ** R.pts_to x #0.5R (v + 1))
+                        (fun _ -> pred (v + 1) ** qpred (v + 1) ** R.pts_to x #0.5R (v + 1))))
+requires L.lock_alive l #p (exists* v. pts_to x #0.5R v ** pred v) ** R.pts_to x #0.5R 'i ** qpred 'i
+ensures  L.lock_alive l #p (exists* v. pts_to x #0.5R v ** pred v) ** R.pts_to x #0.5R ('i + 1) ** qpred ('i + 1)
  {
     let vx = !x;
     rewrite (qpred 'i) as (qpred vx);
     L.acquire l;
     R.gather x;
-    with p v. rewrite (pts_to x #p v) as (pts_to x v);
+    with p v. rewrite (R.pts_to x #p v) as (R.pts_to x v);
     x := (vx + 1);
     R.share x;
-    with p _v. rewrite (pts_to x #p _v) as (pts_to x #one_half _v);
+    with p _v. rewrite (R.pts_to x #p _v) as (R.pts_to x #0.5R _v);
     with _v. rewrite (pred _v) as (pred vx);
     f vx;
     L.release l;
-    with p _v. rewrite (pts_to x #p _v) as (pts_to x #one_half _v);
+    with p _v. rewrite (R.pts_to x #p _v) as (R.pts_to x #0.5R _v);
     rewrite (qpred (vx + 1)) as (qpred ('i + 1));
 }
-```
 
-```pulse
+
+
 fn increment_f2 (x: ref int)
-                (#pred #qpred: int -> vprop)
-                (l:L.lock (exists* v. pts_to x v ** pred v))
-                (f: (v:int -> vq:int -> stt_ghost unit emp_inames 
+                (#p:perm)
+                (#pred #qpred: int -> slprop)
+                (l:L.lock)
+                (f: (v:int -> vq:int -> stt_ghost unit
+                        emp_inames
                         (pred v ** qpred vq ** pts_to x (v + 1))
                         (fun _ -> pred (v + 1) ** qpred (vq + 1) ** pts_to x (v + 1))))
-requires qpred 'i
-ensures qpred ('i + 1)
+requires L.lock_alive l #p (exists* v. pts_to x v ** pred v) ** qpred 'i
+ensures L.lock_alive l #p (exists* v. pts_to x v ** pred v) ** qpred ('i + 1)
  {
     L.acquire l;
     let vx = !x;
@@ -66,10 +87,10 @@ ensures qpred ('i + 1)
     f vx 'i;
     L.release l;
 }
-```
+
 
 #push-options "--warn_error -249"
-```pulse
+
 fn parallel_increment
         (x: ref int)
 requires pts_to x 'i
@@ -83,8 +104,8 @@ ensures pts_to x ('i + 2)
       exists* (v:int).
         pts_to x v **
         (exists* (vl vr:int).
-          GR.pts_to left #(half_perm full_perm) vl **
-          GR.pts_to right #(half_perm full_perm) vr **
+          pts_to left #0.5R vl **
+          pts_to right #0.5R vr **
           pure (v == 'i + vl + vr))
     );
     ghost
@@ -94,56 +115,64 @@ ensures pts_to x ('i + 2)
         (v vq:int)
       requires 
         (exists* (vl vr:int).
-            GR.pts_to left #(half_perm full_perm) vl **
-            GR.pts_to right #(half_perm full_perm) vr **
+            pts_to left #0.5R vl **
+            pts_to right #0.5R vr **
             pure (v == 'i + vl + vr)) **
-        GR.pts_to lr #(half_perm full_perm) vq **
+        pts_to lr #0.5R vq **
         pts_to x (v + 1)
       ensures
         (exists* (vl vr:int).
-            GR.pts_to left #(half_perm full_perm) vl **
-            GR.pts_to right #(half_perm full_perm) vr **
+            pts_to left #0.5R vl **
+            pts_to right #0.5R vr **
             pure (v + 1 == 'i + vl + vr)) **
-        GR.pts_to lr #(half_perm full_perm) (vq + 1) **
+        pts_to lr #0.5R (vq + 1) **
         pts_to x (v + 1)
     { 
       if b
       {
-        with _p _v. rewrite (GR.pts_to lr #_p _v) as (GR.pts_to left #_p _v);
+        with _p _v. rewrite (pts_to lr #_p _v) as (pts_to left #_p _v);
         GR.gather left;
-        with _p _v. rewrite (GR.pts_to left #_p _v) as (GR.pts_to left _v);
+        with _p _v. rewrite (pts_to left #_p _v) as (pts_to left _v);
         GR.( left := vq + 1 );
         GR.share left;      
-        with _p _v. rewrite (GR.pts_to left #_p _v) as (GR.pts_to lr #_p _v);
+        with _p _v. rewrite (pts_to left #_p _v) as (pts_to lr #_p _v);
       }
       else
       {
-        with _p _v. rewrite (GR.pts_to lr #_p _v) as (GR.pts_to right #_p _v);
+        with _p _v. rewrite (pts_to lr #_p _v) as (pts_to right #_p _v);
         GR.gather right;
-        with _p _v. rewrite (GR.pts_to right #_p _v) as (GR.pts_to right _v);
+        with _p _v. rewrite (pts_to right #_p _v) as (pts_to right _v);
         GR.( right := vq + 1 );
         GR.share right;      
-        with _p _v. rewrite (GR.pts_to right #_p _v) as (GR.pts_to lr #_p _v);
+        with _p _v. rewrite (pts_to right #_p _v) as (pts_to lr #_p _v);
       }
     };
 
+    with pred. assert (L.lock_alive lock #1.0R (exists* v. pts_to x v ** pred v));
+    L.share lock;
     parallel
-    requires GR.pts_to left #(half_perm full_perm) 0
-         and GR.pts_to right #(half_perm full_perm) 0
-    ensures  GR.pts_to left #(half_perm full_perm) 1
-         and GR.pts_to right #(half_perm full_perm) 1
+    requires pts_to left #0.5R 0 **
+             L.lock_alive lock #0.5R (exists* v. pts_to x v ** pred v)
+         and pts_to right #0.5R 0 **
+             L.lock_alive lock #0.5R (exists* v. pts_to x v ** pred v)
+    ensures  pts_to left #0.5R 1 **
+             L.lock_alive lock #0.5R (exists* v. pts_to x v ** pred v)
+         and pts_to right #0.5R 1 **
+             L.lock_alive lock #0.5R (exists* v. pts_to x v ** pred v)
     { increment_f2 x lock (step left true) }
     { increment_f2 x lock (step right false) };
 
+    L.gather lock;
     L.acquire lock;
     GR.gather left;
     GR.gather right;
-    with _p _v. rewrite (GR.pts_to left #_p _v) as (GR.pts_to left _v);
-    with _p _v. rewrite (GR.pts_to right #_p _v) as (GR.pts_to right _v);
+    with _p _v. rewrite (pts_to left #_p _v) as (pts_to left _v);
+    with _p _v. rewrite (pts_to right #_p _v) as (pts_to right _v);
     GR.free left;
     GR.free right;
+    L.free lock
 }
-```
+
 
 assume
 val atomic_increment (r:ref int) (#i:erased int)
@@ -151,47 +180,52 @@ val atomic_increment (r:ref int) (#i:erased int)
     (pts_to r i)
     (fun _ -> pts_to r (i + 1))
      
-module F = Pulse.Lib.FlippableInv
 
-let test #p (l:inv p) = assert (not (mem_inv emp_inames l))
-let pts_to_refine #a (x:ref a) (p:a -> vprop) = exists* v. pts_to x v ** p v 
-```pulse
+let test (l:iname) = assert (not (mem_inv emp_inames l))
+let pts_to_refine #a (x:ref a) (p:a -> slprop) = exists* v. pts_to x v ** p v 
+
 fn atomic_increment_f2
         (x: ref int)
-        (#pred #qpred: int -> vprop)
-        (l:inv (pts_to_refine x pred))
-        (f: (v:int -> vq:int -> stt_ghost unit emp_inames 
+        (#pred #qpred: int -> slprop)
+        (l:iname)
+        (f: (v:int -> vq:int -> stt_ghost unit emp_inames
                   (pred v ** qpred vq ** pts_to x (v + 1))
                   (fun _ -> pred (v + 1) ** qpred (vq + 1) ** pts_to x (v + 1))))
-requires qpred 'i
-ensures qpred ('i + 1)
+requires inv l (pts_to_refine x pred) ** qpred 'i
+ensures inv l (pts_to_refine x pred) ** qpred ('i + 1)
 {
+  later_credit_buy 1;
   with_invariants l {
+    later_elim _;
     unfold pts_to_refine;
     with v. _;
     atomic_increment x;
     f v 'i;
     fold pts_to_refine;
+    later_intro (pts_to_refine x pred);
   }
 }
-```
 
-open Pulse.Lib.Stick.Util
+
+open Pulse.Lib.Trade.Util
 module FA = Pulse.Lib.Forall.Util
-module I = Pulse.Lib.Stick.Util
-```pulse
+module I = Pulse.Lib.Trade.Util
+
 fn atomic_increment_f3
         (x: ref int)
-        (#pred #qpred: int -> vprop)
-        (l:inv (pts_to_refine x pred))
+        (#pred #qpred: int -> slprop)
+        (l:iname)
 requires
+  inv l (pts_to_refine x pred) **
   qpred 'i **
   (forall* v vq.
      (pred v ** qpred vq ** pts_to x (v + 1)) @==>
      (pred (v + 1) ** qpred (vq + 1) ** pts_to x (v + 1)))
-ensures qpred ('i + 1)
+ensures inv l (pts_to_refine x pred) ** qpred ('i + 1)
 {
+  later_credit_buy 1;
   with_invariants l {
+    later_elim _;
     unfold pts_to_refine;
     with v. _;
     atomic_increment x;
@@ -202,33 +236,39 @@ ensures qpred ('i + 1)
                            (pred (v + 1) ** qpred (vq + 1) ** pts_to x (v + 1))) 'i;
     I.elim _ _;
     fold pts_to_refine;
+    later_intro (pts_to_refine x pred);
   }
 }
-```
+
 #pop-options
-```pulse
+
 fn atomic_increment_f4
         (x: ref int)
-        (#invp : vprop)
-        (#pred #qpred: int -> vprop)
-        (l:inv invp)
-        (f: (v:int -> vq:int -> stt_ghost unit emp_inames 
+        (#invp : slprop)
+        (#pred #qpred: int -> slprop)
+        (l:iname)
+        (f: (v:int -> vq:int -> stt_ghost unit
+                  emp_inames
                   (pred v ** qpred vq ** pts_to x (v + 1))
                   (fun _ -> pred (v + 1) ** qpred (vq + 1) ** pts_to x (v + 1))))
 requires
+  inv l invp **
   qpred 'i **
   (invp @==> (exists* v. pts_to x v ** pred v)) ** 
   ((exists* v. pts_to x v ** pred v) @==> invp)
-ensures qpred ('i + 1)
+ensures inv l invp ** qpred ('i + 1)
 {
+  later_credit_buy 1;
   with_invariants l {
+    later_elim _;
     I.elim invp _;
     atomic_increment x;
     f _ 'i;
     I.elim (exists* v. pts_to x v ** pred v) invp;
+    later_intro invp;
   }
 }
-```
+
 
 
 assume
@@ -246,36 +286,41 @@ val cas (r:ref int) (u v:int) (#i:erased int)
              (pts_to r i))
 
 
-```pulse
+
 fn atomic_increment_f5
         (x: ref int)
-        (#invp #tok : vprop)
-        (#pred #qpred: int -> vprop)
-        (l:inv invp)
+        (#invp #tok : slprop)
+        (#pred #qpred: int -> slprop)
+        (l:iname)
         (elim_inv: 
           (_:unit -> stt_ghost unit emp_inames invp (fun _ ->
                     ((exists* v. pts_to x v ** pred v) ** tok))))
         (intro_inv:
-            (_:unit -> stt_ghost unit emp_inames 
+            (_:unit -> stt_ghost unit
+                        emp_inames
                         ((exists* v. pts_to x v ** pred v) ** tok)
-                         (fun _ -> invp)))
-        (f: (v:int -> vq:int -> stt_ghost unit emp_inames 
+                        (fun _ -> invp)))
+        (f: (v:int -> vq:int -> stt_ghost unit 
+                  emp_inames
                   (pred v ** qpred vq ** pts_to x (v + 1))
                   (fun _ -> pred (v + 1) ** qpred (vq + 1) ** pts_to x (v + 1))))
-requires qpred 'i
-ensures qpred ('i + 1)
+requires inv l invp ** qpred 'i
+ensures inv l invp ** qpred ('i + 1)
 {
   fn read ()
-  requires emp
+  requires inv l invp
   returns v:int
-  ensures emp
+  ensures inv l invp
   {
+    later_credit_buy 1;
     with_invariants l {
+        later_elim _;
         elim_inv ();
         with i. _;
         let v = atomic_read x;
         rewrite (pts_to x v) as (pts_to x i);
         intro_inv ();
+        later_intro invp;
         v
     }
   };
@@ -288,31 +333,39 @@ ensures qpred ('i + 1)
     b
   )
   invariant b.
+    inv l invp **
     pts_to continue b **
     cond b (qpred 'i) (qpred ('i + 1))
   {
     let v = read ();
+    later_credit_buy 1;
     let next = 
       with_invariants l
       returns b1:bool
-      ensures cond b1 (qpred 'i) (qpred ('i + 1))
+      ensures later invp 
+          ** cond b1 (qpred 'i) (qpred ('i + 1))
           ** pts_to continue true
       {
+        later_elim _;
         elim_inv ();
+        unfold cond;
         let b = cas x v (v + 1);
         if b
         {
-          elim_cond_true b _ _;
-          elim_cond_true true _ _;
-          f _ _;
-          intro_cond_false (qpred 'i) (qpred ('i + 1));
+          unfold cond;
+          with vv. assert (pred vv);
+          f vv _;
           intro_inv ();
+          fold (cond false (qpred 'i) (qpred ('i + 1)));
+          later_intro invp;
           false
         }
         else
         {
-          with p q. rewrite (cond b p q) as q;
+          unfold cond;
           intro_inv ();
+          fold (cond true (qpred 'i) (qpred ('i + 1)));
+          later_intro invp;
           true
         }
       };
@@ -321,33 +374,37 @@ ensures qpred ('i + 1)
   unfold cond;
 }
  
-```
+
 
 module C = Pulse.Lib.CancellableInvariant
 
-```pulse
+
 fn atomic_increment_f6
         (x: ref int)
-        (#p:_) (#t:erased C.token)
-        (#pred #qpred: int -> vprop)
-        (l:inv (C.cancellable t (exists* v. pts_to x v ** pred v)))
-        (f: (v:int -> vq:int -> stt_ghost unit emp_inames 
+        (#p:_)
+        (#pred #qpred: int -> slprop)
+        (c:C.cinv)
+        (f: (v:int -> vq:int -> stt_ghost unit
+                  emp_inames
                   (pred v ** qpred vq ** pts_to x (v + 1))
                   (fun _ -> pred (v + 1) ** qpred (vq + 1) ** pts_to x (v + 1))))
-requires qpred 'i ** C.active p t
-ensures qpred ('i + 1) ** C.active p t
+requires inv (C.iname_of c) (C.cinv_vp c (exists* v. pts_to x v ** pred v)) ** qpred 'i ** C.active c p
+ensures inv (C.iname_of c) (C.cinv_vp c (exists* v. pts_to x v ** pred v)) ** qpred ('i + 1) ** C.active c p
 {
-  with_invariants l {
-    C.take _;
+  later_credit_buy 1;
+  with_invariants (C.iname_of c) {
+    later_elim _;
+    C.unpack_cinv_vp c;
     atomic_increment x;
     f _ 'i;
-    C.restore (exists* v. pts_to x v ** pred v)
+    C.pack_cinv_vp #(exists* v. pts_to x v ** pred v) c;
+    later_intro (C.cinv_vp c (exists* v. pts_to x v ** pred v));
   }
 }
-```
 
 
-```pulse
+
+
 fn parallel_increment_inv
         (x: ref int)
 requires pts_to x 'i
@@ -357,17 +414,15 @@ ensures pts_to x ('i + 2)
     let right = GR.alloc #int 0;
     GR.share left;
     GR.share right;
-    let tok = C.create2 (
+    let c = C.new_cancellable_invariant (
       exists* (v:int).
           pts_to x v **
           (exists* (vl vr:int).
-            GR.pts_to left #(half_perm full_perm) vl **
-            GR.pts_to right #(half_perm full_perm) vr **
+            pts_to left #0.5R vl **
+            pts_to right #0.5R vr **
             pure (v == 'i + vl + vr))
 
     );
-    C.share tok; 
-    let inv = new_invariant' (C.cancellable tok _);
     ghost
     fn step
         (lr:GR.ref int)
@@ -375,59 +430,68 @@ ensures pts_to x ('i + 2)
         (v vq:int)
       requires 
         (exists* (vl vr:int).
-            GR.pts_to left #(half_perm full_perm) vl **
-            GR.pts_to right #(half_perm full_perm) vr **
+            pts_to left #0.5R vl **
+            pts_to right #0.5R vr **
             pure (v == 'i + vl + vr)) **
-        GR.pts_to lr #(half_perm full_perm) vq **
+        pts_to lr #0.5R vq **
         pts_to x (v + 1)
       ensures
         (exists* (vl vr:int).
-            GR.pts_to left #(half_perm full_perm) vl **
-            GR.pts_to right #(half_perm full_perm) vr **
+            pts_to left #0.5R vl **
+            pts_to right #0.5R vr **
             pure (v + 1 == 'i + vl + vr)) **
-        GR.pts_to lr #(half_perm full_perm) (vq + 1) **
+        pts_to lr #0.5R (vq + 1) **
         pts_to x (v + 1)
     { 
       if b
       {
-        with _p _v. rewrite (GR.pts_to lr #_p _v) as (GR.pts_to left #_p _v);
+        with _p _v. rewrite (pts_to lr #_p _v) as (pts_to left #_p _v);
         GR.gather left;
-        with _p _v. rewrite (GR.pts_to left #_p _v) as (GR.pts_to left _v);
+        with _p _v. rewrite (pts_to left #_p _v) as (pts_to left _v);
         GR.( left := vq + 1 );
         GR.share left;      
-        with _p _v. rewrite (GR.pts_to left #_p _v) as (GR.pts_to lr #_p _v);
+        with _p _v. rewrite (pts_to left #_p _v) as (pts_to lr #_p _v);
       }
       else
       {
-        with _p _v. rewrite (GR.pts_to lr #_p _v) as (GR.pts_to right #_p _v);
+        with _p _v. rewrite (pts_to lr #_p _v) as (pts_to right #_p _v);
         GR.gather right;
-        with _p _v. rewrite (GR.pts_to right #_p _v) as (GR.pts_to right _v);
+        with _p _v. rewrite (pts_to right #_p _v) as (pts_to right _v);
         GR.( right := vq + 1 );
         GR.share right;      
-        with _p _v. rewrite (GR.pts_to right #_p _v) as (GR.pts_to lr #_p _v);
+        with _p _v. rewrite (pts_to right #_p _v) as (pts_to lr #_p _v);
       }
     };
 
-    parallel
-    requires GR.pts_to left #(half_perm full_perm) 0 **
-             C.active (half_perm full_perm) tok
-         and GR.pts_to right #(half_perm full_perm) 0 **
-             C.active (half_perm full_perm) tok
-    ensures  GR.pts_to left #(half_perm full_perm) 1 **
-             C.active (half_perm full_perm) tok
-         and GR.pts_to right #(half_perm full_perm) 1 **
-             C.active (half_perm full_perm) tok
-    { atomic_increment_f6 x inv (step left true) }
-    { atomic_increment_f6 x inv (step right false) };
+    C.share c;
+    with pred. assert (inv (C.iname_of c) (C.cinv_vp c (exists* v. pts_to x v ** pred v)));
+    dup_inv (C.iname_of c) (C.cinv_vp c (exists* v. pts_to x v ** pred v));
 
-    C.gather tok;
-    C.cancel_inv inv;
+    parallel
+    requires pts_to left #0.5R 0 **
+             C.active c 0.5R **
+             inv (C.iname_of c) (C.cinv_vp c (exists* v. pts_to x v ** pred v))
+         and pts_to right #0.5R 0 **
+             C.active c 0.5R **
+             inv (C.iname_of c) (C.cinv_vp c (exists* v. pts_to x v ** pred v))
+    ensures  pts_to left #0.5R 1 **
+             C.active c 0.5R **
+             inv (C.iname_of c) (C.cinv_vp c (exists* v. pts_to x v ** pred v))
+         and pts_to right #0.5R 1 **
+             C.active c 0.5R **
+             inv (C.iname_of c) (C.cinv_vp c (exists* v. pts_to x v ** pred v))
+    { atomic_increment_f6 x c (step left true) }
+    { atomic_increment_f6 x c (step right false) };
+
+    C.gather c;
+    drop_ (inv (C.iname_of c) (C.cinv_vp c (exists* v. pts_to x v ** pred v)));
+    later_credit_buy 1;
+    C.cancel c;
     GR.gather left;
     GR.gather right;
-    with _p _v. rewrite (GR.pts_to left #_p _v) as (GR.pts_to left _v);
-    with _p _v. rewrite (GR.pts_to right #_p _v) as (GR.pts_to right _v);
+    with _p _v. rewrite (pts_to left #_p _v) as (pts_to left _v);
+    with _p _v. rewrite (pts_to right #_p _v) as (pts_to right _v);
     GR.free left;
     GR.free right;
-
 }
-```
+
