tutorial/PulseTutorial.Conditionals.fst
@@ -15,12 +15,12 @@
 *)
 
 module PulseTutorial.Conditionals
+#lang-pulse
 open Pulse.Lib.Pervasives
 
-//SNIPPET_START: max$
+//max$
 let max_spec x y = if x < y then y else x
 
-```pulse
 fn max #p #q (x y:ref int)
 requires pts_to x #p 'vx ** pts_to y #q 'vy
 returns n:int
@@ -38,11 +38,10 @@ ensures pts_to x #p 'vx ** pts_to y #q 'vy
         vy
     }
 }
-```
-//SNIPPET_END: max$
+//end max$
 
 [@@expect_failure]
-```pulse //max_alt_fail$
+//max_alt_fail$
 fn max_alt #p #q (x y:ref int)
 requires pts_to x #p 'vx ** pts_to y #q 'vy
 returns n:int
@@ -62,10 +61,10 @@ ensures pts_to x #p 'vx ** pts_to y #q 'vy
     };
     !result;
 }
-```
+//end max_alt_fail$
 
 
-```pulse //max_alt$
+//max_alt$
 fn max_alt #p #q (x y:ref int)
 requires pts_to x #p 'vx ** pts_to y #q 'vy
 returns n:int
@@ -91,25 +90,23 @@ ensures pts_to x #p 'vx ** pts_to y #q 'vy
     };
     !result;
 }
-```
+//end max_alt$
 
 
-module T = FStar.Tactics
-
-//SNIPPET_START: nullable_ref$
+//nullable_ref$
 let nullable_ref a = option (ref a)
 
 let pts_to_or_null #a
         (x:nullable_ref a) 
-        (#[default_arg (`full_perm)] p:perm) //implicit argument with a default
+        (#[default_arg (`1.0R)] p:perm) //implicit argument with a default
         (v:option a)
-: vprop
+: slprop
 = match x with
   | None -> pure (v == None)
   | Some x -> exists* w. pts_to x #p w ** pure (v == Some w)
-//SNIPPET_END: nullable_ref$
+//end nullable_ref$
 
-```pulse //read_nullable$
+//read_nullable$
 fn read_nullable #a #p (r:nullable_ref a)
 requires pts_to_or_null r #p 'v
 returns o:option a
@@ -130,14 +127,14 @@ ensures pts_to_or_null r #p 'v
         unfold (pts_to_or_null None #p 'v);
         fold (pts_to_or_null None #p 'v);
         rewrite each (None #(ref a)) as r;
-        None #a
+        None
      }
     }
 }
-```
+//end read_nullable$
 
-//SNIPPET_START: pts_to_or_null_helpers$
-```pulse
+
+//pts_to_or_null_helpers$
 ghost
 fn elim_pts_to_or_null_none #a #p (r:nullable_ref a)
 requires pts_to_or_null r #p 'v ** pure (r == None)
@@ -148,9 +145,7 @@ ensures pts_to_or_null r #p 'v ** pure ('v == None)
     fold (pts_to_or_null None #p 'v);
     rewrite each (None #(ref a)) as r;
 }
-```
 
-```pulse
 ghost
 fn intro_pts_to_or_null_none #a #p (r:nullable_ref a)
 requires pure (r == None)
@@ -159,9 +154,7 @@ ensures pts_to_or_null r #p None
     fold (pts_to_or_null #a None #p None);
     rewrite each (None #(ref a)) as r;
 }
-```
 
-```pulse
 ghost
 fn elim_pts_to_or_null_some #a #p (r:nullable_ref a) (x:ref a)
 requires pts_to_or_null r #p 'v ** pure (r == Some x)
@@ -170,9 +163,7 @@ ensures exists* w. pts_to x #p w ** pure ('v == Some w)
     rewrite each r as (Some x);
     unfold (pts_to_or_null (Some x) #p 'v);
 }
-```
 
-```pulse
 ghost
 fn intro_pts_to_or_null_some #a #p (r:nullable_ref a) (x:ref a)
 requires pts_to x #p 'v ** pure (r == Some x)
@@ -181,10 +172,9 @@ ensures pts_to_or_null r #p (Some 'v)
     fold (pts_to_or_null (Some x) #p (Some 'v));
     rewrite each (Some x) as r;
 }
-```
-//SNIPPET_END: pts_to_or_null_helpers$
+//end pts_to_or_null_helpers$
 
-```pulse //read_nullable_alt$
+//read_nullable_alt$
 fn read_nullable_alt #a #p (r:nullable_ref a)
 requires pts_to_or_null r #p 'v
 returns o:option a
@@ -193,22 +183,22 @@ ensures pts_to_or_null r #p 'v
 {
     match r {
      Some x -> {
-        elim_pts_to_or_null_some r x;
+        elim_pts_to_or_null_some (Some x) x;
         let o = !x;
         intro_pts_to_or_null_some r x;
         Some o
      }
      None -> {
-        elim_pts_to_or_null_none r;
-        None #a
+        unfold pts_to_or_null None 'v;
+        fold pts_to_or_null None 'v;
+        None
      }
     }
 }
-```
+//end read_nullable_alt$
 
-//SNIPPET_START: read_nullable_alt_fail$
+//read_nullable_alt_fail$
 [@@expect_failure]
-```pulse
 fn read_nullable_alt #a #p (r:nullable_ref a)
 requires pts_to_or_null r #p 'v
 returns o:option a
@@ -225,21 +215,23 @@ ensures emp
         admit() }
     }
 }
-```
-//SNIPPET_END: read_nullable_alt_fail$
+//end read_nullable_alt_fail$
 
-```pulse //write_nullable$
+//write_nullable$
 fn write_nullable #a (r:nullable_ref a) (v:a)
 requires pts_to_or_null r 'v
 ensures exists* w. pts_to_or_null r w ** pure (Some? r ==> w == Some v)
 {
     match r {
-     None -> { () }
+     None -> {
+        rewrite pts_to_or_null None 'v
+             as pts_to_or_null r 'v;
+     }
      Some x -> {
-        elim_pts_to_or_null_some r x;
+        unfold pts_to_or_null (Some x) 'v;
         x := v;
         intro_pts_to_or_null_some r x;
      }
     }
 }
-```
+//end write_nullable$
