tutorial/PulseTutorial.SpinLock.fst
@@ -1,55 +1,94 @@
+(*
+   Copyright 2023 Microsoft Research
+
+   Licensed under the Apache License, Version 2.0 (the "License");
+   you may not use this file except in compliance with the License.
+   You may obtain a copy of the License at
+
+       http://www.apache.org/licenses/LICENSE-2.0
+
+   Unless required by applicable law or agreed to in writing, software
+   distributed under the License is distributed on an "AS IS" BASIS,
+   WITHOUT WARRANTIES OR CONDITIONS OF ANY KIND, either express or implied.
+   See the License for the specific language governing permissions and
+   limitations under the License.
+*)
+
 module PulseTutorial.SpinLock
+#lang-pulse
+
 open Pulse.Lib.Pervasives
-module Box = Pulse.Lib.Box
+
+module B = Pulse.Lib.Box
+
 module U32 = FStar.UInt32
 
 //lock$
-let maybe (b:bool) (p:vprop) =
-    if b then p else emp
+let maybe (b:bool) (p:slprop) =
+  if b then p else emp
 
-let lock_inv (r:ref U32.t) (p:vprop) =
-  exists* v. pts_to r v ** maybe (v = 0ul) p
+let lock_inv (r:B.box U32.t) (p:slprop) : slprop =
+  exists* v. B.pts_to r v ** maybe (v = 0ul) p
 
 noeq
-type lock (p:vprop) = {
-  r:ref U32.t;
-  i:inv (lock_inv r p);
+type lock = {
+  r:B.box U32.t;
+  i:iname;
 }
-//lock$
 
-```pulse //new_lock$
-fn new_lock (p:vprop)
-requires p
-returns l:lock p
-ensures emp
+let lock_alive (l:lock) (p:slprop) =
+  inv l.i (lock_inv l.r p)
+//end lock$
+
+ //dup_lock_alive$
+ghost
+fn dup_lock_alive (l:lock) (p:slprop)
+  requires lock_alive l p
+  ensures lock_alive l p ** lock_alive l p
 {
-   let r = Box.alloc 0ul;
-   Box.to_ref_pts_to r;
+  unfold lock_alive;
+  dup_inv l.i (lock_inv l.r p);
+  fold lock_alive;
+  fold lock_alive
+}
+//end dup_lock_alive$
+
+ //new_lock$
+fn new_lock (p:slprop)
+requires p
+returns l:lock
+ensures lock_alive l p
+{
+   let r = B.alloc 0ul;
    fold (maybe (0ul = 0ul) p);
-   fold (lock_inv (Box.box_to_ref r) p);
-   let i = new_invariant (lock_inv (Box.box_to_ref r) p);
-   let l = { r = Box.box_to_ref r; i };
+   fold (lock_inv r p);
+   let i = new_invariant (lock_inv r p);
+   let l = {r;i};
+   rewrite (inv i (lock_inv r p)) as
+           (inv l.i (lock_inv l.r p));
+   fold lock_alive;
    l
 }
-```
+//end new_lock$
 
 
-
-```pulse
 //acquire_sig$
-fn rec acquire #p (l:lock p)
-requires emp
-ensures p
-//acquire_sig$
+fn rec acquire (#p:slprop) (l:lock)
+requires lock_alive l p
+ensures lock_alive l p ** p
+//end acquire_sig$
 //acquire_body$
 {
+  unfold lock_alive;
+  later_credit_buy 1;
   let b = 
     with_invariants l.i
-    returns b:bool
-    ensures maybe b p 
-    {
+      returns b:bool
+      ensures later (lock_inv l.r p) ** maybe b p
+      opens [l.i] {
+      later_elim _;
       unfold lock_inv;
-      let b = cas l.r 0ul 1ul;
+      let b = cas_box l.r 0ul 1ul;
       if b
       { 
         elim_cond_true _ _ _;
@@ -58,6 +97,7 @@ ensures p
         rewrite (maybe false p) as (maybe (1ul = 0ul) p);
         fold (lock_inv l.r p);
         fold (maybe true p);
+        later_intro (lock_inv l.r p);
         true
       }
       else
@@ -65,26 +105,35 @@ ensures p
         elim_cond_false _ _ _;
         fold (lock_inv l.r p);
         fold (maybe false p);
+        later_intro (lock_inv l.r p);
         false
       }
     };
+  fold lock_alive;
   if b { rewrite (maybe b p) as p; }
   else { rewrite (maybe b p) as emp; acquire l }
 }
-```
+//end acquire_body$
 
-```pulse //release$
-fn release #p (l:lock p)
-requires p
-ensures emp
+//release$
+fn release (#p:slprop) (l:lock)
+requires lock_alive l p ** p
+ensures lock_alive l p
 {
-  with_invariants l.i {
+  unfold lock_alive;
+  later_credit_buy 1;
+  with_invariants l.i
+    returns _:unit
+    ensures later (lock_inv l.r p)
+    opens [l.i] {
+    later_elim _;
     unfold lock_inv;
-    write_atomic l.r 0ul;
-    drop_ (maybe _ _); //double release
+    write_atomic_box l.r 0ul;
+    drop_ (maybe _ _); //maybe release without acquire
     fold (maybe (0ul = 0ul) p);
     fold (lock_inv l.r p);
-  }
+    later_intro (lock_inv l.r p);
+  };
+  fold lock_alive
 }
-```
-
+//end release$
