tutorial/exercises/PulseTutorialExercises.SpinLock3.fst
@@ -2,16 +2,16 @@
    with an additional permission to track when a lock is live,
    so that it can eventually be freed. *)
 module PulseTutorialExercises.SpinLock3
+#lang-pulse
 open Pulse.Lib.Pervasives
-module Box = Pulse.Lib.Box
 module U32 = FStar.UInt32
 module GR = Pulse.Lib.GhostReference
 
 //lock$
-let maybe (b:bool) (p:vprop) =
+let maybe (b:bool) (p:slprop) =
     if b then p else emp
 
-let lock_inv (r:ref U32.t) (live:GR.ref bool) (p:vprop) =
+let lock_inv (r:ref U32.t) (live:GR.ref bool) (p:slprop) =
   exists* b. 
     GR.pts_to live #one_half b **
     maybe b (
@@ -21,7 +21,7 @@ let lock_inv (r:ref U32.t) (live:GR.ref bool) (p:vprop) =
     )
 
 noeq
-type lock (p:vprop) = {
+type lock (p:slprop) = {
   r:ref U32.t;
   live:GR.ref bool;
   i:inv (lock_inv r live p);
@@ -31,7 +31,7 @@ let lock_live #p (l:lock p) (#[default_arg (`full_perm)] perm:perm) =
     GR.pts_to l.live #(half_perm perm) true
 //lock$
 
-```pulse
+
 fn new_lock ()
 requires p
 returns l:lock p
@@ -39,19 +39,19 @@ ensures lock_live l
 {
     admit()
 }
-```
 
 
-```pulse
+
+
 fn free_lock #p (l:lock p)
 requires lock_live l 
 ensures emp
 {
     admit()
 }
-```
 
-```pulse
+
+
 ghost
 fn share #p #q (l:lock p)
 requires lock_live l #q
@@ -59,7 +59,7 @@ ensures lock_live l #(half_perm q) ** lock_live l #(half_perm q)
 {
     admit()
 }
-```
+
 
 let sum_halves (x y:perm)
  : Lemma (ensures sum_perm (half_perm x) (half_perm y) == half_perm (sum_perm x y))
@@ -67,7 +67,7 @@ let sum_halves (x y:perm)
  = let open FStar.Real in
    assert (forall (x y:FStar.Real.real). ( x /. 2.0R ) +. (y /. 2.0R) == ((x +. y) /. 2.0R))
 
-```pulse
+
 ghost
 fn gather #p #q1 #q2 (l:lock p)
 requires lock_live l #q1 ** lock_live l #q2
@@ -75,23 +75,23 @@ ensures lock_live l #(sum_perm q1 q2)
 {
     admit()
 }
-```
 
-```pulse
+
+
 fn acquire #p #q (l:lock p)
 requires lock_live l #q 
 ensures p ** lock_live l #q
 {
     admit()
 }
-```
 
-```pulse
+
+
 fn release #p #q (l:lock p)
 requires p ** lock_live l #q 
 ensures lock_live l #q
 {
     admit()
 }
-```
+
 
