tutorial/solutions/PulseTutorialSolutions.SpinLock2.fst
@@ -1,14 +1,15 @@
 module PulseTutorialSolutions.SpinLock2
+#lang-pulse
 open Pulse.Lib.Pervasives
 module Box = Pulse.Lib.Box
 module U32 = FStar.UInt32
 module GR = Pulse.Lib.GhostReference
 
 //lock$
-let maybe (b:bool) (p:vprop) =
+let maybe (b:bool) (p:slprop) =
     if b then p else emp
 
-let lock_inv (r:ref U32.t) (gr:GR.ref U32.t) (p:vprop) =
+let lock_inv (r:ref U32.t) (gr:GR.ref U32.t) (p:slprop) =
   exists* v perm. 
     pts_to r v **
     GR.pts_to gr #perm v **
@@ -16,7 +17,7 @@ let lock_inv (r:ref U32.t) (gr:GR.ref U32.t) (p:vprop) =
     pure (if v=0ul then perm == full_perm else perm == one_half)
 
 noeq
-type lock (p:vprop) = {
+type lock (p:slprop) = {
   r:ref U32.t;
   gr:GR.ref U32.t;
   i:inv (lock_inv r gr p);
@@ -25,8 +26,8 @@ type lock (p:vprop) = {
 
 let locked #p (l:lock p) = GR.pts_to l.gr #one_half 1ul
 
-```pulse
-fn new_lock (p:vprop)
+
+fn new_lock (p:slprop)
 requires p
 returns l:lock p
 ensures emp
@@ -40,10 +41,10 @@ ensures emp
    let l = { r = Box.box_to_ref r; gr; i };
    l
 }
-```
 
 
-```pulse
+
+
 fn rec acquire #p (l:lock p)
 requires emp
 ensures p ** locked l
@@ -80,9 +81,9 @@ ensures p ** locked l
   if b { with q. rewrite (maybe b q) as q; }
   else { with q. rewrite (maybe b q) as emp; acquire l }
 }
-```
 
-```pulse
+
+
 fn release #p (l:lock p)
 requires p ** locked l
 ensures emp
@@ -100,9 +101,9 @@ ensures emp
   }
 
 }
-```
 
-```pulse
+
+
 fn acquire_loop #p (l:lock p)
 requires emp
 ensures p ** locked l
@@ -153,4 +154,4 @@ ensures p ** locked l
   };
   with _b _q. rewrite (maybe _b _q) as _q;
 }
-```
+
