tutorial/PulseByExample.fst
@@ -16,7 +16,6 @@
 
 module PulseByExample
 
-module PM = Pulse.Main
 open Pulse.Lib.Core
 
 (* 
@@ -27,9 +26,10 @@ open Pulse.Lib.Core
 *)
 
 //SNIPPET_START: five
+#lang-pulse
+
 let fstar_five : int = 5
 
-```pulse
 fn five ()
   requires emp
   returns n:int
@@ -37,12 +37,12 @@ fn five ()
 { 
   fstar_five
 }
-```
+
 
 let pulse_five_in_fstar = five ()
 //SNIPPET_END: five
 
-```pulse
+
 fn five_alt ()
   requires emp
   returns n:(n:int { n == 5 })
@@ -50,7 +50,7 @@ fn five_alt ()
 { 
   5
 }
-```
+
 
 open Pulse.Lib.Reference
 module R = Pulse.Lib.Reference
@@ -62,7 +62,7 @@ module R = Pulse.Lib.Reference
   - default full permission
   - heap reference, read and write
 *)
-```pulse
+
 fn ref_swap (r1 r2:ref int)
   requires
     R.pts_to r1 'n1 **
@@ -77,7 +77,7 @@ fn ref_swap (r1 r2:ref int)
   r1 := v2;
   r2 := v1
 }
-```
+
 
 open Pulse.Lib.Array
 module A = Pulse.Lib.Array
@@ -91,7 +91,7 @@ open Pulse.Lib.BoundedIntegers
   - machine integers, ops on bounded integers
 *)
 
-```pulse
+
 fn arr_swap (#t:Type0) (n i j:SZ.t) (a:larray t (v n))
   requires
     A.pts_to a 's0 **
@@ -109,7 +109,7 @@ fn arr_swap (#t:Type0) (n i j:SZ.t) (a:larray t (v n))
   a.(i) <- vj;
   a.(j) <- vi;
 }
-```
+
 
 (* 
   Things to note:
@@ -117,7 +117,7 @@ fn arr_swap (#t:Type0) (n i j:SZ.t) (a:larray t (v n))
   - mutable local reference, read and write
   - variable permission
 *)
-```pulse
+
 fn max (n:SZ.t) (a:larray nat (v n))
   requires
     A.pts_to a #'p 's **
@@ -156,10 +156,10 @@ fn max (n:SZ.t) (a:larray nat (v n))
   let vmax = !max;
   vmax
 }
-```
-// This option may become the default at some point
+
+//this option should become the default, once I shake out the handling of address-taking
 #push-options "--ext 'pulse:rvalues'"
-```pulse
+
 fn max_alt (n:SZ.t) (a:larray nat (v n))
   requires
     A.pts_to a #'p 's **
@@ -189,5 +189,18 @@ fn max_alt (n:SZ.t) (a:larray nat (v n))
   };
   max
 }
-```
+
 #pop-options
+
+(* 
+- some more mature example (e.g. sorting alg)
+
+- some simple record data structure along with a library of functions on this DS
+  (e.g. library of functions on 2D points)
+
+- build up to explaining the pulse implementation of lpht? -- emphasis on connecting
+  pure implementation to imperative code
+- pulse linked list? -- more traditional sep logic example 
+
+- concurrency, e.g. par incr of a ctr
+*)
