tutorial/PulseTutorial.AtomicsAndInvariants.fst
@@ -1,40 +1,99 @@
+(*
+   Copyright 2023 Microsoft Research
+
+   Licensed under the Apache License, Version 2.0 (the "License");
+   you may not use this file except in compliance with the License.
+   You may obtain a copy of the License at
+
+       http://www.apache.org/licenses/LICENSE-2.0
+
+   Unless required by applicable law or agreed to in writing, software
+   distributed under the License is distributed on an "AS IS" BASIS,
+   WITHOUT WARRANTIES OR CONDITIONS OF ANY KIND, either express or implied.
+   See the License for the specific language governing permissions and
+   limitations under the License.
+*)
+
 module PulseTutorial.AtomicsAndInvariants
+#lang-pulse
 open Pulse.Lib.Pervasives
+module T = FStar.Tactics
 module U32 = FStar.UInt32
 
 //owns$
-let owns (x:ref U32.t) = exists* v. pts_to x v
-//owns$
+let owns (x:ref U32.t) : timeless_slprop = exists* v. pts_to x v
+//end owns$
 
-```pulse //create_invariant$
+//owns_timeless$
+let owns_timeless (x:ref U32.t)
+: squash (timeless (owns x))
+by T.(norm [delta_only [`%owns; `%auto_squash]]; 
+      mapply (`FStar.Squash.return_squash);
+      mapply (`timeless_exists))
+= ()
+//end owns_timeless$
+
+//create_invariant$
+ghost
 fn create_invariant (r:ref U32.t) (v:erased U32.t)
 requires pts_to r v
-returns i:inv (owns r)
-ensures emp
+returns i:iname
+ensures inv i (owns r)
 {
     fold owns;
     new_invariant (owns r)
 }
-```
+//end create_invariant$
 
-let singleton #p (i:inv p) = add_inv emp_inames i
-
-```pulse //update_ref_atomic$
+//update_ref_atomic0$
+[@@expect_failure]
 atomic
-fn update_ref_atomic (r:ref U32.t) (i:inv (owns r)) (v:U32.t)
-requires emp
-ensures emp
-opens (singleton i)
+fn update_ref_atomic (r:ref U32.t) (i:iname) (v:U32.t)
+requires inv i (owns r)
+ensures inv i (owns r)
 {
-  with_invariants i {    //owns r
+  with_invariants i {    //later (owns r)
+     unfold owns;        //cannot prove owns; only later (owns r)
+  }
+}
+//end update_ref_atomic0$
+
+
+//update_ref_atomic$
+atomic
+fn update_ref_atomic (r:ref U32.t) (i:iname) (v:U32.t)
+requires inv i (owns r) ** later_credit 1
+ensures inv i (owns r)
+opens [i]
+{
+  with_invariants i {    //later (owns r) ** later_credit 1
+     later_elim _;       //ghost step: owns r
      unfold owns;        //ghost step;  exists* u. pts_to r u
      write_atomic r v;   //atomic step; pts_to r v
      fold owns;          //ghost step;  owns r
-  }
+     later_intro (owns r) //ghost step: later (owns r)
+  } // inv i (owns r)
 }
-```
+//end update_ref_atomic$
 
-```pulse
+//update_ref_atomic_alt$
+atomic
+fn update_ref_atomic_alt (r:ref U32.t) (i:iname) (v:U32.t)
+requires inv i (owns r)
+ensures inv i (owns r)
+opens [i]
+{
+  with_invariants i {    //later (owns r) ** later_credit 1
+     later_elim_timeless _;       //owns r
+     unfold owns;        //ghost step;  exists* u. pts_to r u
+     write_atomic r v;   //atomic step; pts_to r v
+     fold owns;          //ghost step;  owns r
+     later_intro (owns r) //later (owns r)
+  } // inv i (owns r)
+}
+//end update_ref_atomic_alt$
+
+
 ghost
 fn pts_to_dup_impossible #a (x:ref a)
 requires pts_to x 'v ** pts_to x 'u
@@ -44,11 +103,10 @@ ensures  pts_to x 'v ** pts_to x 'u ** pure False
     pts_to_perm_bound x;
     share x;    
 }
-```
+
 
 //double_open_bad$
 [@@expect_failure]
-```pulse
 fn double_open_bad (r:ref U32.t) (i:inv (owns r))
 requires emp
 ensures pure False
@@ -63,29 +121,23 @@ ensures pure False
       }
     }
 }
-```
-//double_open_bad$
+//end double_open_bad$
 
-
-```pulse //update_ref$
-fn update_ref (r:ref U32.t) (i:inv (owns r)) (v:U32.t)
-requires emp
-ensures emp
+//update_ref$
+fn update_ref (r:ref U32.t) (i:iname) (v:U32.t)
+requires inv i (owns r)
+ensures inv i (owns r)
 {                    
-  with_invariants i {    //owns r
-     unfold owns;        //ghost step;  exists* u. pts_to r u
-     write_atomic r v;   //atomic step; pts_to r v
-     fold owns;          //ghost step;  owns r
-  }
+  later_credit_buy 1;
+  update_ref_atomic r i v;
 }
-```
+//end update_ref$
 
 //update_ref_fail$
-[@@expect_failure]
-```pulse 
-fn update_ref_fail (r:ref U32.t) (i:inv (owns r)) (v:U32.t)
-requires emp
-ensures emp
+[@@expect_failure] 
+fn update_ref_fail (r:ref U32.t) (i:iname) (v:U32.t)
+requires inv i (owns r)
+ensures inv i (owns r)
 {
   with_invariants i {
     unfold owns;
@@ -93,28 +145,37 @@ ensures emp
     fold owns;
   }
 }
-```
-//update_ref_fail$
+//end update_ref_fail$
+
+let readable (r:ref U32.t) : timeless_slprop  = exists* p v. pts_to r #p v
+
+ghost
+fn intro_readable (r:ref U32.t) (p:perm) (v:U32.t)
+  requires pts_to r #p v
+  ensures  readable r
+{
+  fold readable
+}
 
 
-
-let readable (r:ref U32.t) = exists* p v. pts_to r #p v
-
-```pulse //split_readable$
-atomic
-fn split_readable (r:ref U32.t) (i:inv (readable r))
-requires emp
-ensures readable r
-opens (singleton i)
+//split_readable$
+ghost
+fn split_readable (r:ref U32.t) (i:iname)
+requires inv i (readable r)
+ensures inv i (readable r) ** readable r
+opens [i]
 {
     with_invariants i {
+        later_elim_timeless _;
         unfold readable;
+        with p v. assert (pts_to r #p v);
         share r;
-        fold readable;
-        fold readable;
+        (* just folding readable would now be ambiguous, need the explicit intro. *)
+        // fold readable;
+        // fold readable;
+        intro_readable r (p /. 2.0R) _;
+        intro_readable r (p /. 2.0R) _;
+        later_intro (readable r)
     };
 }
-```
-
-
-
+//end split_readable$
