tutorial/PulseTutorial.HigherOrder.fst
@@ -1,11 +1,28 @@
+(*
+   Copyright 2023 Microsoft Research
+
+   Licensed under the Apache License, Version 2.0 (the "License");
+   you may not use this file except in compliance with the License.
+   You may obtain a copy of the License at
+
+       http://www.apache.org/licenses/LICENSE-2.0
+
+   Unless required by applicable law or agreed to in writing, software
+   distributed under the License is distributed on an "AS IS" BASIS,
+   WITHOUT WARRANTIES OR CONDITIONS OF ANY KIND, either express or implied.
+   See the License for the specific language governing permissions and
+   limitations under the License.
+*)
+
 module PulseTutorial.HigherOrder
+#lang-pulse
 open Pulse.Lib.Pervasives
-module B = Pulse.Lib.Box
-```pulse //apply$
+
+//apply$
 fn apply (#a:Type0)
          (#b:a -> Type0)
-         (#pre:a -> vprop)
-         (#post: (x:a -> b x -> vprop))
+         (#pre:a -> slprop)
+         (#post: (x:a -> b x -> slprop))
          (f: (x:a -> stt (b x) (pre x) (fun y -> post x y)))
          (x:a)
 requires pre x
@@ -14,15 +31,16 @@ ensures post x y
 {
   f x
 }
-```
+//end apply$
 
-```pulse //apply_ghost$
+
+//apply_ghost$
 ghost
 fn apply_ghost 
          (#a:Type0)
          (#b:a -> Type0)
-         (#pre:a -> vprop)
-         (#post: (x:a -> b x -> vprop))
+         (#pre:a -> slprop)
+         (#post: (x:a -> b x -> slprop))
          (f: (x:a -> stt_ghost (b x) emp_inames (pre x) (fun y -> post x y)))
          (x:a)
 requires pre x
@@ -31,55 +49,34 @@ ensures post x y
 {
   f x
 }
-```
+//end apply_ghost$
+
 
 let id_t = (#a:Type0) -> x:a -> stt a emp (fun _ -> emp)
 
-```pulse
 fn id ()
 : id_t 
 = (#a:Type0) (x:a) { x }
-```
 
 let id_t_a (a:Type0) = x:a -> stt a emp (fun _ -> emp)
 
-[@@expect_failure] //FIXME! This should work!
-```pulse
 fn id_a (a:Type0)
 : id_t_a a 
 = (x:a) { x }
-```
-
-```pulse
-fn id_a (a:Type0)
-requires emp
-returns f:id_t_a a 
-ensures emp
-{
-  fn aux (x:a)
-  requires emp
-  returns y:a
-  ensures emp 
-  { 
-    x 
-};
-  aux
-}
-```
 
 
 //ctr$
 noeq
 type ctr = {
-    inv: int -> vprop;
+    inv: int -> slprop;
     next: i:erased int -> stt int (inv i) (fun y -> inv (i + 1) ** pure (y == reveal i));
     destroy: i:erased int -> stt unit (inv i) (fun _ -> emp)
 }
-//ctr$
+//end ctr$
 let next c = c.next
 let destroy c = c.destroy
 
-```pulse //new_counter$
+//new_counter$
 fn new_counter ()
 requires emp
 returns c:ctr
@@ -106,9 +103,8 @@ ensures c.inv 0
     rewrite (pts_to x 0) as (c.inv 0);
     c
 }
-```
+//end new_counter$
 
-```pulse
 fn return (#a:Type0) (x:a)
 requires emp
 returns y:a
@@ -116,19 +112,21 @@ ensures pure (x == y)
 {
     x
 }
-```
 
 
-```pulse //test_counter$
+
+//test_counter$
 fn test_counter ()
 requires emp
 ensures emp
 {
     let c = new_counter ();
-    let x = next c _; //FIXME: Should be able to write c.next
+    let next = c.next;
+    let destroy = c.destroy;
+    let x = next _; //FIXME: Should be able to write c.next
     assert pure (x == 0);
-    let x = next c _;
+    let x = next _;
     assert pure (x == 1);
-    destroy c _;
+    destroy _;
 }
-```
+//end test_counter$
