tutorial/PulseTutorial.Intro.fst
@@ -15,11 +15,12 @@
 *)
 
 module PulseTutorial.Intro
+#lang-pulse
 open Pulse.Lib.Pervasives
 
 
 
-```pulse
+
 fn par (#p #q #r #s:_)
        (f: (unit -> stt unit p (fun _ -> q)))
        (g: (unit -> stt unit r (fun _ -> s)))
@@ -33,11 +34,11 @@ ensures q ** s
         { g () };
     ()
 }
-```
+
 
 let incr_functional (x:int) = x + 1
 
-```pulse //incr
+//incr$
 fn incr (x:ref int)
 requires pts_to x 'i
 ensures pts_to x ('i + 1)
@@ -45,9 +46,9 @@ ensures pts_to x ('i + 1)
     let v = !x;
     x := v + 1;
 }
-```
+//end incr$
 
-```pulse //incr_explicit_i
+//incr_explicit_i$
 fn incr_explicit_i (x:ref int) (i:erased int)
 requires pts_to x i
 ensures pts_to x (i + 1)
@@ -55,10 +56,9 @@ ensures pts_to x (i + 1)
     let v = !x;
     x := v + 1;
 }
-```
+//end incr_explicit_i$
 
-
-```pulse //par_incr
+//par_incr$
 fn par_incr (x y:ref int)
 requires pts_to x 'i ** pts_to y 'j
 ensures pts_to x ('i + 1) ** pts_to y ('j + 1)
@@ -66,23 +66,23 @@ ensures pts_to x ('i + 1) ** pts_to y ('j + 1)
    par (fun _ -> incr x)
        (fun _ -> incr y)
 }
-```
+//end par_incr$
 
-```pulse //incr_frame
+
+//incr_frame$
 fn incr_frame (x y:ref int)
 requires pts_to x 'i ** pts_to y 'j
 ensures pts_to x ('i + 1) ** pts_to y 'j
 {
    incr x;
 }
-```
+//end incr_frame$
 
-```pulse //incr_frame_any
-fn incr_frame_any (x:ref int) (f:vprop)
+//incr_frame_any$
+fn incr_frame_any (x:ref int) (f:slprop)
 requires pts_to x 'i ** f
 ensures pts_to x ('i + 1) ** f
 {
    incr x;
 }
-```
-
+//end incr_frame_any$
